Several improvements.

theories/lang/wise_prophet.v
@@ -44,6 +44,14 @@ Section wise_prophet.
   Implicit Types γ_full γ_past : gname.
   Implicit Types prophs : prophecies.
 
+  Definition wise_prophet_full γ_full full :=
+    agree_on γ_full full.
+
+  Definition wise_prophet_past_auth γ_past past :=
+    mono_list_auth γ_past 1 past.
+  Definition wise_prophet_past_lb γ_past past_lb :=
+    mono_list_lb γ_past past_lb.
+
   Definition wise_prophet_model γ_model prophs :=
     auth_excl_auth γ_model (DfracOwn 1) prophs.
 
@@ -51,10 +59,15 @@ Section wise_prophet.
     ∃ past prophs,
     typed_prophet_model prophet p prophs ∗
     auth_excl_frag γ_model prophs ∗
-    agree_on γ_full (past ++ prophs) ∗
-    mono_list_auth γ_past 1 past.
+    wise_prophet_full γ_full (past ++ prophs) ∗
+    wise_prophet_past_auth γ_past past.
   Definition wise_prophet_inv p γ_model γ_full γ_past ι :=
     inv ι (wise_prophet_inv_inner p γ_model γ_full γ_past).
+
+  Definition wise_prophet_lb γ_full γ_past lb : iProp Σ :=
+    ∃ past_lb,
+    wise_prophet_full γ_full (past_lb ++ lb) ∗
+    wise_prophet_past_lb γ_past past_lb.
 
   #[global] Instance wise_prophet_model_timeless γ_model prophs :
     Timeless (wise_prophet_model γ_model prophs).
@@ -66,6 +79,16 @@ Section wise_prophet.
   Proof.
     apply _.
   Qed.
+  #[global] Instance wise_prophet_lb_timeless γ_full γ_past lb :
+    Timeless (wise_prophet_lb γ_full γ_past lb).
+  Proof.
+    apply _.
+  Qed.
+  #[global] Instance wise_prophet_lb_persistent γ_full γ_past lb :
+    Persistent (wise_prophet_lb γ_full γ_past lb).
+  Proof.
+    apply _.
+  Qed.
 
   Lemma wise_prophet_model_exclusive p prophs1 prophs2 :
     wise_prophet_model p prophs1 -∗
@@ -73,6 +96,67 @@ Section wise_prophet.
     False.
   Proof.
     apply auth_excl_auth_exclusive.
+  Qed.
+
+  Lemma wise_prophet_inv_acc p γ_model γ_full γ_past ι E :
+    ↑ι ⊆ E →
+    wise_prophet_inv p γ_model γ_full γ_past ι ={E, E ∖ ↑ι}=∗
+      ∃ past prophs,
+      wise_prophet_full γ_full (past ++ prophs) ∗
+      wise_prophet_past_auth γ_past past ∗
+      (wise_prophet_past_auth γ_past past ={E ∖ ↑ι, E}=∗ True).
+  Proof.
+    iIntros "% #Hinv".
+    iMod (inv_acc with "Hinv") as "((%past & %prophs & >Hp & >Hmodel₂ & >#Hfull & >Hpast_auth) & Hclose)"; first done.
+    iModIntro. iExists past, prophs. iFrame "#∗". iIntros "Hpast_auth".
+    iApply "Hclose". iNext. iExists past, prophs. iFrame "#∗".
+  Qed.
+
+  Lemma wise_prophet_lb_get γ_full γ_past past prophs :
+    wise_prophet_full γ_full (past ++ prophs) -∗
+    wise_prophet_past_auth γ_past past -∗
+    wise_prophet_lb γ_full γ_past prophs.
+  Proof.
+    iIntros "Hfull Hpast_auth".
+    iExists past. iFrame. iApply (mono_list_lb_get with "Hpast_auth").
+  Qed.
+  Lemma wise_prophet_lb_get' p γ_model γ_full γ_past ι prophs E :
+    ↑ι ⊆ E →
+    wise_prophet_inv p γ_model γ_full γ_past ι -∗
+    wise_prophet_model γ_model prophs ={E}=∗
+      wise_prophet_model γ_model prophs ∗
+      wise_prophet_lb γ_full γ_past prophs.
+  Proof.
+    iIntros "% #Hinv Hmodel₁".
+    iInv "Hinv" as "(%past & %_prophs & >Hp & >Hmodel₂ & >#Hfull & >Hpast_auth)".
+    iDestruct (auth_excl_agree_L with "Hmodel₁ Hmodel₂") as %<-.
+    iDestruct (wise_prophet_lb_get with "Hfull Hpast_auth") as "#$".
+    iModIntro. iFrame. iSplitL; last done. iExists past, prophs. iFrame "#∗".
+  Qed.
+  Lemma wise_prophet_lb_suffix γ_full γ_past past prophs lb :
+    wise_prophet_full γ_full (past ++ prophs) -∗
+    wise_prophet_past_auth γ_past past -∗
+    wise_prophet_lb γ_full γ_past lb -∗
+    ⌜prophs `suffix_of` lb⌝.
+  Proof.
+    iIntros "Hfull Hpast_auth (%past_lb & Hfull' & Hpast_lb)".
+    iDestruct (agree_on_agree_L with "Hfull Hfull'") as %Hfull.
+    iDestruct (mono_list_auth_lb_valid with "Hpast_auth Hpast_lb") as %(_ & past_delta & ->).
+    iPureIntro. rewrite -assoc in Hfull. solve_suffix.
+  Qed.
+  Lemma wise_prophet_lb_suffix' p γ_model γ_full γ_past ι prophs lb E :
+    ↑ι ⊆ E →
+    wise_prophet_inv p γ_model γ_full γ_past ι -∗
+    wise_prophet_model γ_model prophs -∗
+    wise_prophet_lb γ_full γ_past lb ={E}=∗
+      wise_prophet_model γ_model prophs ∗
+      ⌜prophs `suffix_of` lb⌝.
+  Proof.
+    iIntros "% #Hinv Hmodel₁ Hlb".
+    iInv "Hinv" as "(%past & %_prophs & >Hp & >Hmodel₂ & >#Hfull & >Hpast_auth)".
+    iDestruct (auth_excl_agree_L with "Hmodel₁ Hmodel₂") as %<-.
+    iDestruct (wise_prophet_lb_suffix with "Hfull Hpast_auth Hlb") as "#$".
+    iModIntro. iFrame. iSplitL; last done. iExists past, prophs. iFrame "#∗".
   Qed.
 
   Lemma wise_prophet_new_proph_spec ι E :
@@ -88,7 +172,7 @@ Section wise_prophet.
     iApply wp_fupd. wp_apply (typed_prophet_new_proph_spec with "[//]"). iIntros "%p %prophs Hp".
     iMod (auth_excl_alloc' prophs) as "(%γ_model & Hmodel₁ & Hmodel₂)".
     iMod (agree_alloc prophs) as "(%γ_full & #Hfull)".
-    iMod (mono_list_alloc []) as "(%γ_past & Hpast & _)".
+    iMod (mono_list_alloc []) as "(%γ_past & Hpast_auth & _)".
     iApply "HΦ". iFrame. iApply inv_alloc. iNext. iExists [], prophs. auto with iFrame.
   Qed.
 
@@ -100,11 +184,11 @@ Section wise_prophet.
     wise_prophet_model γ_model prophs -∗
     WP e @ E ∖ ↑ι {{ w,
       ∀ past,
-      agree_on γ_full (past ++ prophs) -∗
-      mono_list_auth γ_past 1 past ={E ∖ ↑ι}=∗
+      wise_prophet_full γ_full (past ++ prophs) -∗
+      wise_prophet_past_auth γ_past past ={E ∖ ↑ι}=∗
         ∃ proph,
         ⌜(w, v) = prophet.(typed_prophet_to_val) proph⌝ ∗
-        mono_list_auth γ_past 1 past ∗
+        wise_prophet_past_auth γ_past past ∗
           ∀ prophs',
           ⌜prophs = proph :: prophs'⌝ -∗
           wise_prophet_model γ_model prophs' ={E ∖ ↑ι}=∗
@@ -113,19 +197,41 @@ Section wise_prophet.
     WP Resolve e #p v @ E {{ Φ }}.
   Proof.
     iIntros "% % % Hinv Hmodel₁ HΦ".
-    iInv "Hinv" as "(%past & %_prophs & >Hp & >Hmodel₂ & >#Hfull & >Hpast)"; first apply strongly_atomic_atomic, _.
+    iInv "Hinv" as "(%past & %_prophs & >Hp & >Hmodel₂ & >#Hfull & >Hpast_auth)"; first apply strongly_atomic_atomic, _.
     iDestruct (auth_excl_agree_L with "Hmodel₁ Hmodel₂") as %<-.
     wp_apply (typed_prophet_resolve_spec with "Hp"); first done.
     iApply wp_fupd. wp_apply (wp_wand with "HΦ"). iIntros "%w HΦ".
-    iMod ("HΦ" with "Hfull Hpast") as "(%proph & % & Hpast & HΦ)".
+    iMod ("HΦ" with "Hfull Hpast_auth") as "(%proph & % & Hpast_auth & HΦ)".
     iModIntro. iExists proph. iSplitR; first done. iIntros "%prophs' -> Hp".
     iMod (auth_excl_update' prophs' with "Hmodel₁ Hmodel₂") as "(Hmodel₁ & Hmodel₂)".
-    iMod (mono_list_auth_update_app [proph] with "Hpast") as "(Hpast & _)".
+    iMod (mono_list_auth_update_app [proph] with "Hpast_auth") as "(Hpast_auth & _)".
     iMod ("HΦ" with "[//] Hmodel₁") as "$".
     iModIntro. iNext. iExists (past ++ [proph]), prophs'. iFrame. list_simplifier. done.
+  Qed.
+  Lemma wise_prophet_resolve_spec' e v E p γ_model γ_full γ_past ι prophs Φ :
+    ↑ι ⊆ E →
+    Atomic StronglyAtomic e →
+    to_val e = None →
+    wise_prophet_inv p γ_model γ_full γ_past ι -∗
+    wise_prophet_model γ_model prophs -∗
+    WP e @ E ∖ ↑ι {{ w,
+      ∃ proph,
+      ⌜(w, v) = prophet.(typed_prophet_to_val) proph⌝ ∗
+        ∀ prophs',
+        ⌜prophs = proph :: prophs'⌝ -∗
+        wise_prophet_model γ_model prophs' ={E ∖ ↑ι}=∗
+        Φ w
+    }} -∗
+    WP Resolve e #p v @ E {{ Φ }}.
+  Proof.
+    iIntros "% % % Hinv Hmodel₁ HΦ".
+    wp_apply (wise_prophet_resolve_spec with "Hinv Hmodel₁"); [done.. |].
+    wp_apply (wp_wand with "HΦ"). iIntros "%w (%proph & % & HΦ) %past _ Hpast_auth".
+    iModIntro. iExists proph. iFrame. done.
   Qed.
 End wise_prophet.
 
 #[global] Opaque wise_prophet_name.
 #[global] Opaque wise_prophet_model.
 #[global] Opaque wise_prophet_inv.
+#[global] Opaque wise_prophet_lb.
